HuffmanAlgorithm/BasicLemmas.lean
@@ -6,36 +6,40 @@ import Mathlib.Tactic
 This file contains basic lemmas about element of finset and their intersections
 
 It provides results showing that if two sets are disjoint:
-
 - An element cannot belong to both sets at the same time.
 - Membership in one set means non-membership in the other.
 -/
 
+/--
+If `A` and `B` are disjoint (their intersection is empty),
+no element can belong to both sets at the same time.
+-/
 lemma mem_inter_empty {α} [DecidableEq α]
   (A B : Finset α) (a : α) (h : A ∩ B = ∅)
   (h1 : a ∈ A) (h2 : a ∈ B) : False := by
   have : a ∈ A ∩ B := Finset.mem_inter_of_mem h1 h2
   simp [h] at this
 
-lemma not_mem_right_of_inter_empty {α} [DecidableEq α]
+lemma not_mem_right {α} [DecidableEq α]
   {A B : Finset α} {a : α} :
   A ∩ B = ∅ → a ∈ A → a ∉ B := by
   intro h ha hb
   have : a ∈ A ∩ B := Finset.mem_inter.mpr ⟨ha, hb⟩
   simp [h] at this
 
-lemma not_mem_left_of_inter_empty {α} [DecidableEq α]
+lemma not_mem_left {α} [DecidableEq α]
   {A B : Finset α} {a : α} :
   A ∩ B = ∅ → a ∈ B → a ∉ A := by
   intro h ha hb
   have : a ∈ A ∩ B := Finset.mem_inter.mpr ⟨hb, ha⟩
   simp [h] at this
 
+/--
+If `A` and `B` are disjoint,
+- `a` in `A` means `a` not in `B`
+- `a` in `B` means `a` not in `A`.
+-/
 lemma not_mem_inter_empty {α} {A B : Finset α} {a : α} [DecidableEq α] :
   A ∩ B = ∅ → (a ∈ A → a ∉ B) ∧ (a ∈ B → a ∉ A) := by
   intro h
-  constructor <;> intro ha hb
-  · have : a ∈ A ∩ B := Finset.mem_inter.mpr ⟨ha, hb⟩
-    simp [h] at this
-  · have : a ∈ A ∩ B := Finset.mem_inter.mpr ⟨hb, ha⟩
-    simp [h] at this
+  constructor <;> grind[mem_inter_empty]
